@prefix rdfs: <http://www.w3.org/2000/01/rdf-schema#>.
@prefix owl2xml: <http://www.w3.org/2006/12/owl2-xml#>.
@prefix xsd: <http://www.w3.org/2001/XMLSchema#>.
@prefix schema: <http://prov4j.org/w3p/schema#>.
@prefix owl: <http://www.w3.org/2002/07/owl#>.
@prefix rdf: <http://www.w3.org/1999/02/22-rdf-syntax-ns#>.
@prefix vann:     <http://purl.org/vocab/vann/> .

@prefix foaf:     <http://xmlns.com/foaf/0.1/> .
@prefix dcterms:  <http://purl.org/dc/terms/> .
@prefix opmo:   <http://openprovenance.org/model/opmo#>.
@prefix cc: <http://creativecommons.org/ns#>.
@prefix void: <http://rdfs.org/ns/void#> .
@prefix frbr: <http://purl.org/vocab/frbr/core#>.

# --- Own namespaces ------------------------------------------

@prefix lex:        <http://purl.org/lex#> .
@prefix lexm:        <http://purl.org/lex/meta#> .
@prefix lexdt:        <http://purl.org/lex/datatypes#> .
@prefix lexissuertypes: <http://purl.org/lex/lex-issuer-types#> .
@prefix lexsoltypes: <http://purl.org/lex/lex-sol-types#> .

# --- Ontology metadata ---------------------------------------

lex: a owl:Ontology ;
  dcterms:title "Lex ontology"@en ;
  dcterms:description "Lex ontology."@en ;
  dcterms:modified "2012-10-21"^^xsd:date ;
  vann:preferredNamespaceUri "http://purl.org/lex#" ;
  vann:preferredNamespacePrefix "lex" ;
  dcterms:creator <http://purl.org/knap#me>;
  rdfs:seeAlso <http://prefix.cc/lex> ;
  dcterms:rights <http://creativecommons.org/licenses/by/3.0/cz/> .


##########
## Classes
########

# Defines the particular source of law classes for Work, Expression, Manifestation
lex:SourceOfLaw a owl:Class ;
	rdfs:label "Právní zdroj"@cs, "Source of law"@en ;
	rdfs:comment "Tøída reprezentující právní zdroj (zákon, vyhláška, judikát)"@cs ;
  rdfs:comment "A class representing a source of law (law, notice, case law)."@en ;
	rdfs:subClassOf frbr:Work .
	
lex:SourceOfLawExpression a owl:Class ;
	rdfs:label "Znìní právního zdroje"@cs, "Source of law expression"@en ;
	rdfs:comment "Tøída reprezentující znìní právního zdroje. Každý právní zdroj mùže mít nìkolik znìní. Napø. zákon mùže mít pùvodní znìní a potom nìkolik novelizovaná znìní."@cs ;
  rdfs:comment "A class representing expression of the source of law. A source of law may have several expressions. E.g., a law may have its original expression and then several revised expressions."@en ;
	rdfs:subClassOf frbr:Expression .
	
lex:SourceOfLawManifestation a owl:Class ;
	rdfs:label "Materializovaná forma znìní právního zdroje "@cs, "Manifestation of a source of law expression"@en ;
	rdfs:comment "Tøída reprezentující znìní právního zdroje materializované v podobì nìjakého konkrétního dokumentu v konkrétním formátu (napø. PDF)."@cs ;
  rdfs:comment "A class representing source of law materialized in a form of a concrete document in a concrete format (e.g., PDF)."@en ;
	rdfs:subClassOf frbr:Manifestation .

# Defines sections
# Valid for Acts, Notices, not for Judgements! (TODO how to express explicitely?)
# the first one is used to denote all sections, regardless if it is a section of Work, Expression, or Manifestation
lex:SourceOfLawSectionInGeneral a owl:Class ;
	rdfs:label "Paragraf právního zdroje"@cs, "Section in general"@en ;
	rdfs:comment "A class representing a general section."@en .
lex:SourceOfLawSection a owl:Class ;
	rdfs:label "Paragraf právního zdroje"@cs, "Section of work"@en ;
	rdfs:comment "A class representing section of a Work."@en ;
	rdfs:subClassOf lex:SourceOfLawSectionInGeneral .
lex:SourceOfLawExpressionSection a owl:Class ;
	rdfs:label "Paragraf znìní právního zdroje"@cs, "Section of expression"@en ;
	rdfs:comment "A class representing section of a Expression."@en ;
	rdfs:subClassOf lex:SourceOfLawSectionInGeneral .
lex:SourceOfLawManifestationSection a owl:Class ;
	rdfs:label "Paragraf reprezentace znìní právního zdroje"@cs, "Section of expression's manifestation"@en ;
	rdfs:comment "A class representing section of a Manifestation."@en ;
	rdfs:subClassOf lex:SourceOfLawSectionInGeneral .

##########
## Object Properties
########

# to associate lex:SourceOfLaw with lex:SourceOfLawExpression 
# goal: to relate source of law with its first and last expression)
lex:lastExpression a owl:FunctionalProperty;
	rdfs:label "Poslední znìní"@cs, "Last expression"@en ;
	rdfs:comment "Last expression of the Work"@en ;
	rdfs:domain lex:SourceOfLaw;
	rdfs:range lex:SourceOfLawExpression.
lex:originalExpression a owl:FunctionalProperty;
	rdfs:label "Pùvodní znìní"@cs, "Original expression"@en ;
	rdfs:comment "Original expression of the Work"@en ;
	rdfs:domain lex:SourceOfLaw;
	rdfs:range lex:SourceOfLawExpression.

# to associate lex:SourceOfLaw with another lex:SourceOfLaw or lex:SourceOfLawExpression 
# goal: to express novelization (high level view)
# TODO tyka se Act, Notice - should be restricted to Act, Notice as sourceOfLawType?
lex:amends a owl:ObjectProperty;
	rdfs:label "Novelizuje"@cs, "Amends"@en ;
	rdfs:comment "A Work amends/novelizes another Work"@en ;
	rdfs:domain lex:SourceOfLaw;
	rdfs:range lex:SourceOfLaw.
lex:sourceOfAmendment a owl:ObjectProperty;
	rdfs:label "Zdroj novelizace"@cs, "Source of amendment"@en ;
	rdfs:comment "A Work points to another Expression being a source of amendment"@en ;
	rdfs:domain lex:SourceOfLaw;
	rdfs:range lex:SourceOfLawExpression.
lex:targetOfAmendment a owl:ObjectProperty;
	rdfs:label "Novelizované znìní"@cs, "Target of amendment"@en ;
	rdfs:comment "A Work points to another Expression being a target of amendment"@en ;
	rdfs:domain lex:SourceOfLaw;
	rdfs:range lex:SourceOfLawExpression.

	
# to associate lex:SourceOfLawSection with another lex:SourceOfLawSection 
# goal: to express novelization (low level view) - to expresses that one section creates, removes, modifies another one
# should be restricted to Act, Notice as sourceOfLawType (TODO)
lex:createsSection a owl:ObjectProperty;
	rdfs:label "Pøidává paragraf"@cs, "Creates section"@en ;
	rdfs:comment "A section of Work (novel) creates certain section in another Work (novelized Work)"@en ;
	rdfs:domain lex:SourceOfLawSection;
	rdfs:range lex:SourceOfLawSection .	
#can be infered from lex:createsSection and lex:targetOfAmendment 
#TODO chceme to?
lex:created a owl:ObjectProperty;
	rdfs:label "Pragraf pøidán"@cs, "Section created"@en ;
	rdfs:comment "A section of Work (novel) points to the section of Expression which was created by applying that novel"@en ;
	rdfs:domain lex:SourceOfLawSection;
	rdfs:range lex:SourceOfLawExpressionSection .

lex:removesSection a owl:ObjectProperty;
	rdfs:label "Ruší "@cs, "Amends"@en ;
	rdfs:comment "A section of Work (novel) removes certain section in another Work (novelized Work)"@en ;
	rdfs:domain lex:SourceOfLawSection ;
	rdfs:range lex:SourceOfLawSection .
#can be infered from lex:removesSection and lex:sourceOfAmendment 
#TODO chceme to?
lex:removed a owl:ObjectProperty;
	rdfs:label "Pragraf odebrán"@cs, "Section removed"@en ;
	rdfs:comment "A section of Work (novel) points to the section of Expression which was removed by applying that novel"@en ;
	rdfs:domain lex:SourceOfLawSection;
	rdfs:range lex:SourceOfLawExpressionSection .
	
lex:modifiesSection a owl:ObjectProperty;
	rdfs:label "Upravuje paragraf"@cs, "Modifies section"@en ;
	rdfs:comment "A section of Work (novel) modifies certain section in another Work (novelized Work)"@en ;
	rdfs:domain lex:SourceOfLawSection ;
	rdfs:range lex:SourceOfLawSection .	 
#can be infered from modifiesSection and lex:sourceOfAmendment 
#TODO chceme to?
lex:originalSection a owl:ObjectProperty;
	rdfs:label "Pùvodní paragraf"@cs, "Original section"@en ;
	rdfs:comment "A section of Work (novel) points to the section before the modification of the expression to which the novel applies"@en ;
	rdfs:domain lex:SourceOfLawSection;
	rdfs:range lex:SourceOfLawExpressionSection .
#can be infered from modifiesSection and lex:targetOfAmendment 
#TODO chceme to?
lex:modifiedSection a owl:ObjectProperty;
	rdfs:label "Modifikovaný nový paragraf"@cs, "Section modified"@en ;
	rdfs:comment "A section of Work (novel) points to the newly modified section in the expression resulting from the application of the novel"@en ;
	rdfs:domain lex:SourceOfLawSection;
	rdfs:range lex:SourceOfLawExpressionSection .

# to express that Section belongs to Work/Expression/Manifestation
lex:belongsTo a owl:ObjectProperty;
	rdfs:label "je souèástí právního zdroje"@cs, "Is part of source of law"@en ;
	rdfs:comment "A section points the the whole source of law"@en ;
	rdfs:domain lex:SourceOfLawSection;
	rdfs:range lex:SourceOfLaw.
lex:belongsToExpression a owl:ObjectProperty;
	rdfs:label "je souèástí znìní"@cs, "Is part of source of law expression"@en ;
	rdfs:comment "A section points the the whole source of law expression"@en ;
	rdfs:domain lex:SourceOfLawExpressionSection;
	rdfs:range lex:SourceOfLawExpression.	
lex:belongsToManifestation a owl:ObjectProperty;
	rdfs:label "je souèástí reprezentace znìní"@cs, "Is part of source of law manifestation"@en ;
	rdfs:comment "A section points the the whole source of law manifestation"@en ;
	rdfs:domain lex:SourceOfLawManifestationSection;
	rdfs:range lex:SourceOfLawManifestation.

# to express hierarchy of sections 
# TODO how to ensure that only section of work can belong to section of work?
# TODO nebo pouzit dcterms:isPartOf? 
lex:enclosingSection a owl:ObjectProperty;
	rdfs:label "patøí do sekce"@cs, "Enclosing section"@en ;
	rdfs:comment "A section points the section to which it belongs"@en ;
	rdfs:domain lex:SourceOfLawSectionInGeneral;
	rdfs:range lex:SourceOfLawSectionInGeneral.
	
	
	
##########
## Data Properties
########






