@prefix rdfs: <http://www.w3.org/2000/01/rdf-schema#> .
@prefix owl2xml: <http://www.w3.org/2006/12/owl2-xml#> .
@prefix xsd: <http://www.w3.org/2001/XMLSchema#> .
@prefix schema: <http://prov4j.org/w3p/schema#> .
@prefix owl: <http://www.w3.org/2002/07/owl#> .
@prefix rdf: <http://www.w3.org/1999/02/22-rdf-syntax-ns#> .
@prefix vann:     <http://purl.org/vocab/vann/> .

@prefix foaf:     <http://xmlns.com/foaf/0.1/> .
@prefix dcterms:  <http://purl.org/dc/terms/> .
@prefix opmo:   <http://openprovenance.org/model/opmo#> .
@prefix cc: <http://creativecommons.org/ns#> .
@prefix void: <http://rdfs.org/ns/void#> .
@prefix frbr: <http://purl.org/vocab/frbr/core#> .

# --- Own namespaces ------------------------------------------

@prefix lex:        <http://purl.org/lex#> .
@prefix lexm:        <http://purl.org/lex/meta#> .
@prefix lexdt:        <http://purl.org/lex/datatypes#> .
@prefix lexissuertypes: <http://purl.org/lex/lex-issuer-types#> .
#@prefix lexsoltypes: <http://purl.org/lex/lex-sol-types#> .

# --- Ontology metadata ---------------------------------------

lex: a owl:Ontology ;
  dcterms:title "LEX ontology"@en ;
  dcterms:description "LEX ontology models various kinds of sources of law. It is based on various FRBR concepts, namely frbr:Work, frbr:Expression and frbr:Manifestation. "@en ;
  dcterms:modified "2012-11-28"^^xsd:date ;
  vann:preferredNamespaceUri "http://purl.org/lex#" ;
  vann:preferredNamespacePrefix "lex" ;
  dcterms:creator <http://purl.org/knap#me>, <http://purl.org/necasky#me>, <http://purl.org/klimek#me>;
  rdfs:seeAlso <http://prefix.cc/lex> ;
  dcterms:rights <http://creativecommons.org/licenses/by/3.0/cz/> .

##########
## Classes
########

lex:SourceOfLaw a owl:Class ;
	rdfs:label "Právní zdroj"@cs, "Source of law"@en ;
	rdfs:comment "Instance této tøídy reprezentuje právní zdroj (zákon, vyhláška, judikát). Je komplementární ke slovníku FRBR. Používá se pro specifikaci typu dané instance frbr:Work, frbr:Expression èi frbr:Manifestation, která reprezentuje zákon, vyhlášku nebo judikát."@cs ;
  rdfs:comment "An instance of this class represents a source of law (act, notice, court decision). It is independent on FRBR vocabulary. It is used to specifz a type of a given instance of frbr:Work, frbr:Expression or frbr:Manifestation which represents an act, notice or court decitions."@en .
  
lex:Act a owl:Class ;
  rdfs:label "Zákon"@cs, "Law"@en ;
  rdfs:comment "Pokud instance tøídy frbr:Work, frbr:Expression èi frbr:Manifestation reprezentuje zákon, potom je oznaèena i jako instance této tøídy."@cs ;
  rdfs:comment "If an instance of class frbr:Work, frbr:Expression èi frbr:Manifestation represents a law then it is marked also as an instance of this class."@en ;
  rdfs:subClassOf lex:SourceOfLaw .

lex:Decision a owl:Class ;
  rdfs:label "Rozhodnutí soudu"@cs, "Court decision"@en ;
  rdfs:comment "Pokud instance tøídy frbr:Work, frbr:Expression èi frbr:Manifestation reprezentuje rozhodnutí soudu (napø. judikát), potom je oznaèena i jako instance této tøídy."@cs ;
  rdfs:comment "If an instance of class frbr:Work, frbr:Expression èi frbr:Manifestation represents a court decision then it is marked also as an instance of this class."@en ;
  rdfs:subClassOf lex:SourceOfLaw .

lex:Notice a owl:Class ;
  rdfs:label "Vyhláška"@cs, "Notice"@en ;
  rdfs:comment "Pokud instance tøídy frbr:Work, frbr:Expression èi frbr:Manifestation reprezentuje vyhlášku, potom je oznaèena i jako instance této tøídy."@cs ;
  rdfs:comment "If an instance of class frbr:Work, frbr:Expression èi frbr:Manifestation represents a notice then it is marked also as an instance of this class."@en ;
  rdfs:subClassOf lex:SourceOfLaw .
  
lex:Amendment a owl:Class ;
  rdfs:label "Novela"@cs, "Amendment"@en ;
  rdfs:comment "Pokud instance tøídy frbr:Work, frbr:Expression èi frbr:Manifestation reprezentuje novelu, potom je oznaèena i jako instance této tøídy."@cs ;
  rdfs:comment "If an instance of class frbr:Work, frbr:Expression èi frbr:Manifestation represents a amendment then it is marked also as an instance of this class."@en ;
  rdfs:subClassOf lex:Act .

lex:Change a owl:Class ;
  rdfs:label "Zmìna právního zdroje"@cs, "Change of a source of law"@en ;
  rdfs:comment "Právní zdroje (pøedevším zákony) mohou být novelizovány. Novela specifikuje množinu konkrétních jednotlivých zmìn. Ty jsou reprezentovány jako instance této tøídy. Z pohledu FRBR ontologie jsou úpravy provádìny na úrovni frbr:Expression."@cs ;
  rdfs:comment "Sources of law (especially acts) can be amended. An amendment specifies a set of concrete particular changes. The changes are represented as instances of this class. From the point of view of FRBR ontology, amendments are made at the level of frbr:Expression."@en .

lex:Creation a owl:Class ;
  rdfs:label "Vytvoøení nové èásti právního zdroje"@cs, "Creation of a new part of a source of law"@en ;
  rdfs:comment "Instance této tøídy je speciálním typem konkrétní jednotlivé zmìny znamenající vytvoøení nové souèásti právního zdroje."@cs ;
  rdfs:comment "An instance of this class represents a special type of a concrete particular amendment specifying creation of a new part of a source of law."@en ;
  rdfs:subClassOf lex:Creation .

lex:Removal a owl:Class ;
  rdfs:label "Odstranìní existující èásti právního zdroje"@cs, "Removal of an existing part of a source of law"@en ;
  rdfs:comment "Instance této tøídy je speciálním typem konkrétní jednotlivé zmìny znamenající smazání existujícíc souèásti právního zdroje."@cs ;
  rdfs:comment "An instance of this class represents a special type of a concrete particular amendment specifying removal of an existing part of a source of law."@en ;
  rdfs:subClassOf lex:Creation .
  
lex:Update a owl:Class ;
  rdfs:label "Zmìna existující èásti právního zdroje"@cs, "Update of an existing part of a source of law"@en ;
  rdfs:comment "Instance této tøídy je speciálním typem konkrétní jednotlivé zmìny znamenající zmìnu existující souèásti právního zdroje."@cs ;
  rdfs:comment "An instance of this class represents a special type of a concrete particular amendment specifying an update of an existing part of a source of law."@en ;
  rdfs:subClassOf lex:Creation .

lex:Reference a owl:Class ;
  rdfs:label "Reference mezi dvìma právními zdroji"@cs, "A reference between two sources of law"@en ;
  rdfs:comment "Instance této tøídy reprezentuje referenci znìní jednoho právního zdroje na znìní jiného právního zdroje. Umožòuje pøesnì specifikovat i místo výskytu reference v textové reprezentaci odkazujícího se znìní."@cs ;
  rdfs:comment "An instance of this class represents a reference of an expression of one source of law to an expression of another source of law. It enables to exactly specify the occurrence of the reference in the textual representation of the referencing expression." 

##########
## Object Properties
########

lex:lastExpression a owl:FunctionalProperty;
	rdfs:label "Poslední existující znìní právního zdroje"@cs, "Last existing expression of a source of law"@en ;
	rdfs:comment "An instance of this property links the last existing expression with a source of law. The expression exists but it may be the case that it has not come into force yet."@en ;
	# [TODO] domain constraint : frbr:Work && lex:SourceOfLaw 
	rdfs:domain frbr:Work ;
	rdfs:range frbr:Expression .
	
lex:actualExpression a owl:FunctionalProperty;
	rdfs:label "V souèasnosti platné znìní právního zdroje"@cs, "Currently valid expression of a source of law"@en ;
	rdfs:comment "An instance of this property links the currently valid expression with a source of law. This expression does not have to be the last expression."@en ;
	# [TODO] domain constraint : frbr:Work && lex:SourceOfLaw 
	rdfs:domain frbr:Work ;
	rdfs:range frbr:Expression .
	
lex:originalExpression a owl:FunctionalProperty;
	rdfs:label "Pùvodní znìní právního zdroje"@cs, "Original expression of a source of law"@en ;
	rdfs:comment "An instance of this property links the original existing expression with a source of law."@en ;
	# [TODO] domain constraint : frbr:Work && lex:SourceOfLaw 
	rdfs:domain frbr:Work ;
	rdfs:range frbr:Expression .

lex:definesChange a owl:FunctionalProperty;
	rdfs:label "Zmìna definovaná novelou"@cs, "A change defined by an amendment"@en ;
	rdfs:comment "An instance of this property associates an amendment with a particular change defined by the amendment."@en ;
	# [TODO] domain constraint : frbr:Expression && lex:Amendment
	rdfs:domain frbr:Expression ;
	rdfs:range lex:Change .

lex:createsExpression a owl:FunctionalProperty;
	rdfs:label "Vytvoøená èást právního zdroje"@cs, "A newly created part of a source of law"@en ;
	rdfs:comment "An instance of this property associates a creation change with the created part of a source of law."@en ;
	rdfs:domain lex:Removal ;
	# [TODO] range constraint : frbr:Expression && lex:Act && lex:Notice
	rdfs:range frbr:Expression .
	
lex:removesExpression a owl:FunctionalProperty;
	rdfs:label "Vyjmutá èást právního zdroje"@cs, "A removed part of a source of law"@en ;
	rdfs:comment "An instance of this property associates a removal change with the removed part of a source of law."@en ;
	rdfs:domain lex:Removal ;
	# [TODO] range constraint : frbr:Expression && lex:Act && lex:Notice
	rdfs:range frbr:Expression .
	
lex:updatesSourceExpression a owl:FunctionalProperty;
	rdfs:label "Znìní upravované èásti právního zdroje pøed úpravou"@cs, "An expression of an updated part of a source of law before the update"@en ;
	rdfs:comment "An instance of this property associates an update change with the updated part of a source of law before the udpate itself."@en ;
	rdfs:domain lex:Removal ;
	# [TODO] range constraint : frbr:Expression && lex:Act && lex:Notice
	rdfs:range frbr:Expression .
	
lex:updatesTargetExpression a owl:FunctionalProperty;
	rdfs:label "Znìní upravované èásti právního zdroje po úpravì"@cs, "An expression of an updated part of a source of law after the update"@en ;
	rdfs:comment "An instance of this property associates an update change with the updated part of a source of law after the udpate."@en ;
	rdfs:domain lex:Removal ;
	# [TODO] range constraint : frbr:Expression && lex:Act && lex:Notice
	rdfs:range frbr:Expression .

lex:referencingExpression a owl:ObjectProperty;
	rdfs:label "Odkazující se znìní právního zdroje"@cs, "A referencing expression of a source of law"@en ;
	rdfs:comment "An instance of this property links a reference to a referencing expression of a source of law"@en ;
	rdfs:domain lex:Reference;
	# [TODO] range constraint : frbr:Expression && lex:SourceOfLaw
	rdfs:range frbr:Expression .
	
lex:referencedExpression a owl:ObjectProperty;
	rdfs:label "Odkazované znìní právního zdroje"@cs, "A referenced expression of a source of law"@en ;
	rdfs:comment "An instance of this property links a reference to a referenced expression of a source of law"@en ;
	rdfs:domain lex:Reference ;
	# [TODO] range constraint : (frbr:Expression && lex:SourceOfLaw) || lex:Court || ...
	rdfs:range frbr:Expression .
	
##########
## Data Properties
########

lex:startPosition a owl:DataTypeProperty;
  rdfs:label "Poèátek reference ve znìní právního zdroje"@cs, "The start of a reference in an expression of a source of law"@en ;
  rdfs:comment "Poèátek reference je zaznamenán v podobì poøadí prvního znaku reference (první znak má poøadové èíslo 1)."@cs ;
  rdfs:comment "The start of a reference is recorded as an order of the first character of the reference (the order of the first character is 1)."@en ;
  rdfs:domain lex:Reference ;
  rdfs:range xsd:positiveInteger . 
  
lex:endPosition a owl:DataTypeProperty;
  rdfs:label "Konec reference ve znìní právního zdroje"@cs, "The end of a reference in an expression of a source of law"@en ;
  rdfs:comment "Poèátek reference je zaznamenán v podobì poøadí prvního znaku reference."@cs ;
  rdfs:comment "The end of a reference is recorded as an order of the last character of the reference."@en ;
  rdfs:domain lex:Reference ;
  rdfs:range xsd:positiveInteger .






